Cslib/Computability/Automata/EpsilonNA/Basic.lean
@@ -47,7 +47,7 @@ that trace from the start state. -/
 @[scoped grind =]
 instance : Acceptor (FinAcc State Symbol) Symbol where
     Accepts (a : FinAcc State Symbol) (xs : List Symbol) :=
-  ∃ s ∈ a.start, ∃ s' ∈ a.accept, a.SMTr s xs s'
+  ∃ s ∈ a.start, ∃ s' ∈ a.accept, a.SMTr s (xs.map Option.some) s'
 
 end FinAcc
 
